Got rid of slower scaffolding, serialize positives with two constructors per byte

SerializerRewrite.v
@@ -261,7 +261,7 @@ Qed.
 
 Hint Rewrite @fold_append_unwrap @fold_append_unwrap' : cheerios.
 
-(* positive strong induction *)
+(* positive *)
 
 Inductive le_pos (p : positive) : positive -> Prop :=
 | le_p : le_pos p p
@@ -304,213 +304,79 @@ Section PositiveInductionPrinciple.
     now apply strongind_pos_aux.
   Qed.
 End PositiveInductionPrinciple.
-  (* positive serializer *)
 
 Local Open Scope char_scope.
 
-Inductive positive_compressed :=
-| xH'
-| xO' : positive_compressed -> positive_compressed
-| xI' : positive_compressed -> positive_compressed
-| xOxO : positive_compressed -> positive_compressed
-| xOxI : positive_compressed -> positive_compressed
-| xIxO : positive_compressed -> positive_compressed
-| xIxI : positive_compressed -> positive_compressed.
-
-Fixpoint compress_positive_rec (p : positive)
-         (k : positive_compressed -> positive_compressed) :=
+Fixpoint serialize_positive p :=
   match p with
-  | xI (xI p) => compress_positive_rec p (fun c => k (xIxI c))
-  | xI (xO p) => compress_positive_rec p (fun c => k (xIxO c))
-  | xO (xI p) => compress_positive_rec p (fun c => k (xOxI c))
-  | xO (xO p) => compress_positive_rec p (fun c => k (xOxO c))
-  | xI p => compress_positive_rec p (fun c => k (xI' c))
-  | xO p => compress_positive_rec p (fun c => k (xO' c))
-  | xH => k xH'
+  | xI (xI p) => Serializer.append (serialize "000")
+                                   (serialize_positive p)
+  | xI (xO p) => Serializer.append (serialize "001")
+                                   (serialize_positive p)
+  | xO (xI p) => Serializer.append (serialize "002")
+                                   (serialize_positive p)
+  | xO (xO p) => Serializer.append (serialize "003")
+                                   (serialize_positive p)
+  | xI p => Serializer.append (serialize "004")
+                              (serialize_positive p)
+  | xO p => Serializer.append (serialize "005")
+                              (serialize_positive p)
+  | XH => serialize "006"
   end.
 
-Fixpoint compress_positive p :=
-  match p with
-  | xI (xI p) => xIxI (compress_positive p)
-  | xI (xO p) => xIxO (compress_positive p)
-  | xO (xI p) => xOxI (compress_positive p)
-  | xO (xO p) => xOxO (compress_positive p)
-  | xI p => xI' (compress_positive p)
-  | xO p => xO' (compress_positive p)
-  | xH => xH'
-  end.
-
-Definition compress_positive' p :=
-  compress_positive_rec p (fun c => c).
-
-Definition compress_spec (p : positive) :=
-  forall k, compress_positive_rec p k = k (compress_positive p).
-  
-Lemma compress_positive_rec_spec :
-  forall p, compress_spec p.
-Proof.
-  apply strongind_pos;
-    unfold compress_spec in *;
-    intros.
-  - reflexivity.
-  - split;
-      intros;
-      destruct q;
-      intros;
-      simpl;
-      try reflexivity;
-      rewrite H;
-      try reflexivity;
-      repeat constructor.
-Qed.
-
-Fixpoint decompress_positive_rec (c : positive_compressed) (k : positive -> positive) :=
-  match c with
-  | xIxI c => decompress_positive_rec c (fun p => k (xI (xI p)))
-  | xIxO c => decompress_positive_rec c (fun p => k (xI (xO p)))
-  | xOxI c => decompress_positive_rec c (fun p => k (xO (xI p)))
-  | xOxO c => decompress_positive_rec c (fun p => k (xO (xO p)))
-  | xI' c => decompress_positive_rec c (fun p => k (xI p))
-  | xO' c => decompress_positive_rec c (fun p => k (xO p))
-  | xH' => k xH
-  end.
-
-Fixpoint decompress_positive c :=
-  match c with
-  | xIxI c => xI (xI (decompress_positive c))
-  | xIxO c => xI (xO (decompress_positive c))
-  | xOxI c => xO (xI (decompress_positive c))
-  | xOxO c => xO (xO (decompress_positive c))
-  | xI' c => xI (decompress_positive c)
-  | xO' c => xO (decompress_positive c)
-  | xH' => xH
-  end.
-
-Definition decompress_positive' c :=
-  decompress_positive_rec c (fun p => p).
-
-Lemma decompress_positive_rec_spec : forall c k,
-    decompress_positive_rec c k = k (decompress_positive c).
-Proof.
-  induction c;
-    try reflexivity;
-    intros;
-    unfold decompress_positive_rec; fold decompress_positive_rec;
-      unfold decompress_positive; fold decompress_positive;
-        apply IHc.
-Qed.
-
-Lemma compress_decompress_id : forall p,
-    decompress_positive (compress_positive p) = p.
-Proof.
-  apply strongind_pos.
-  - reflexivity.
-  - split;
-      destruct q;
-      intros;
-      simpl;
-      try reflexivity;
-      intros;
-      simpl;
-      assert ((decompress_positive (compress_positive q)) = q);
-      ((apply H; 
-        repeat constructor) || now rewrite H0).
-Qed.
-
-Lemma compress'_decompress'_id : forall p,
-    decompress_positive' (compress_positive' p) = p.
-Proof.
-  intros.
-  unfold decompress_positive', compress_positive'.
-  rewrite decompress_positive_rec_spec, compress_positive_rec_spec.
-  apply compress_decompress_id.
-Qed.
-  
-
-Fixpoint serialize_positive_compressed (p : positive_compressed) : Serializer.t :=
-  match p with
-  | xIxI p => Serializer.append (serialize "000")
-                                   (serialize_positive_compressed p)
-  | xIxO p => Serializer.append (serialize "001")
-                                   (serialize_positive_compressed p)
-  | xOxI p => Serializer.append (serialize "002")
-                                   (serialize_positive_compressed p)
-  | xOxO p => Serializer.append (serialize "003")
-                                   (serialize_positive_compressed p)
-  | xI' p => Serializer.append (serialize "004")
-                              (serialize_positive_compressed p)
-  | xO' p => Serializer.append  (serialize "005")
-                               (serialize_positive_compressed p)
-  | xH' => serialize "006"
-  end.
-
-Definition deserialize_positive_compressed_step
+Definition deserialize_positive_step
            (b : ascii)
-           (s : positive_compressed -> positive_compressed) := 
+           (s : positive -> positive) := 
   if ascii_eq b "000"
-  then More (fun p => s (xIxI p))
+  then More (fun p => s (xI (xI p)))
   else if ascii_eq b "001"
-  then More (fun p => s (xIxO p))
+  then More (fun p => s (xI (xO p)))
        else if ascii_eq b "002"
-            then More (fun p => s (xOxI p))
+            then More (fun p => s (xO (xI p)))
             else if ascii_eq b "003"
-                 then More (fun p => s (xOxO p))
+                 then More (fun p => s (xO (xO p)))
                  else if ascii_eq b "004"
-                      then More (fun p => s (xI' p))
+                      then More (fun p => s (xI p))
                       else if ascii_eq b "005"
-                           then More (fun p => s (xO' p))
+                           then More (fun p => s (xO p))
                            else if ascii_eq b "006"
-                                then Done (s xH')
+                                then Done (s xH)
                                 else Error.
 
-Definition deserialize_positive_compressed : Deserializer.t positive_compressed :=
-  Deserializer.fold deserialize_positive_compressed_step (fun p => p).
+Definition positive_step_aux p :=
+  forall (k : positive -> positive) (bytes : list ascii),
+    Deserializer.unwrap (Deserializer.fold deserialize_positive_step k)
+                        (Serializer.unwrap (serialize_positive p) ++ bytes)
+    = Some(k p, bytes).
 
-Lemma positive_compressed_step :
-  forall (c : positive_compressed)
-         (k : positive_compressed -> positive_compressed)
-         (bytes : list ascii),
-    Deserializer.unwrap (Deserializer.fold deserialize_positive_compressed_step k)
-                        (Serializer.unwrap (serialize_positive_compressed c) ++ bytes)
-    = Some(k c, bytes).
+Lemma positive_step :
+  forall (p : positive), positive_step_aux p.
 Proof.
-  induction c;
-    intros;
-    unfold serialize_positive_compressed;
-    fold serialize_positive_compressed;
-    cheerios_crush;
-    simpl;
-    now rewrite IHc.
+  apply strongind_pos; unfold positive_step_aux.
+  -  unfold serialize_positive.
+    cheerios_crush.
+  - split;
+      intros;
+      destruct q;
+      simpl;
+      cheerios_crush;
+      simpl;
+      try rewrite H;
+      try reflexivity;
+      repeat constructor;
+      cheerios_crush.
 Qed.
-
-Theorem serialize_deserialize_positive_compressed_id :
-  serialize_deserialize_id_spec serialize_positive_compressed
-                                deserialize_positive_compressed.
-Proof.
-  intros.
-  unfold deserialize_positive_compressed.
-  apply positive_compressed_step.
-Qed.
-
-Instance positive_compressed_Serializer : Serializer positive_compressed :=
-  {| serialize := serialize_positive_compressed;
-     deserialize := deserialize_positive_compressed;
-     serialize_deserialize_id :=
-       serialize_deserialize_positive_compressed_id |}.
-
-Definition serialize_positive p :=
-  serialize (compress_positive' p).
 
 Definition deserialize_positive :=
-  Deserializer.map decompress_positive' deserialize.
+  Deserializer.fold deserialize_positive_step (fun p => p).
 
 Theorem serialize_deserialize_positive_id :
-  serialize_deserialize_id_spec serialize_positive deserialize_positive.
+  serialize_deserialize_id_spec serialize_positive
+                                deserialize_positive.
 Proof.
   intros.
-  unfold serialize_positive, deserialize_positive.
-  cheerios_crush.
-  now rewrite compress'_decompress'_id.
+  unfold deserialize_positive.
+  apply positive_step.
 Qed.
 
 Instance positive_Serializer : Serializer positive.
@@ -564,6 +430,7 @@ Proof.
   cheerios_crush.
   now rewrite Nnat.Nat2N.id.
 Qed.
+Check Nnat.Nat2N.id.
 
 Instance nat_Serializer : Serializer nat :=
   {| serialize := serialize_nat;
